Cslib/Logics/Propositional/NaturalDeduction/Theorems.lean
@@ -20,12 +20,12 @@ open Derivation
 /-!
 ### Negation theorems
 
-The following are valid in minimal logic, so we use `impl (-) C` over `~(-) := impl (-) bot`.
+The following are valid in minimal logic, so we use `(-) ⟶ C` over `~(-)`.
 -/
 
 /-- Double negation introduction -/
-def Derivation.dni {A B : Proposition Atom} : Derivation ⟨{A}, impl (impl A B) B⟩ :=
-  implI (A := A.impl B) _ <|
+def Derivation.dni {A B : Proposition Atom} : Derivation ⟨{A}, (A ⟶ B) ⟶ B⟩ :=
+  implI (A := A ⟶ B) _ <|
   implE (A := A) (ax' (by grind)) (ax' (by grind))
 
 theorem SDerivable.dni {A B : Proposition Atom} : SDerivable ⟨{A},impl (impl A B) B⟩ :=
@@ -33,45 +33,45 @@ theorem SDerivable.dni {A B : Proposition Atom} : SDerivable ⟨{A},impl (impl A
 
 /-- The double negation of excluded-middle, or in minimal-logic-style ⊢ (A ∨ (A → B)) → B → B. -/
 def Derivation.notNotLEM {A B : Proposition Atom} :
-    Derivation ⟨∅, (A.disj <| impl A B).impl B |>.impl B⟩ :=
+    Derivation ⟨∅, (A ⋎ (A ⟶ B) ⟶ B) ⟶ B⟩ :=
   implI _ <|
-  implE (A := A.disj (A.impl B)) (ax' <| by grind) <|
+  implE (A := A ⋎ (A ⟶ B)) (ax' <| by grind) <|
   disjI₂ <|
   implI _ <|
-  implE (A := A.disj (A.impl B)) (ax' <| by grind) <|
+  implE (A := A ⋎ (A ⟶ B)) (ax' <| by grind) <|
   disjI₁ <|
   ax' <| by grind
 
 theorem Derivable.not_not_lem {A B : Proposition Atom} :
-    Derivable <| ((A.disj <| impl A B).impl B).impl B :=
+    ⊢ ((A ⋎ (A ⟶ B) ⟶ B) ⟶ B) :=
   derivable_iff.mpr ⟨Derivation.notNotLEM⟩
 
 /-- Triple negation elimination -/
 def Derivation.tne {A B : Proposition Atom} :
-    Derivation ⟨{((A.impl B).impl B).impl B}, A.impl B⟩ :=
+    Derivation ⟨{((A ⟶ B) ⟶ B) ⟶ B}, A ⟶ B⟩ :=
   implI _ <|
-  implE (A := (A.impl B).impl B) (ax' <| by grind) <|
+  implE (A := (A ⟶ B) ⟶ B) (ax' <| by grind) <|
   Derivation.dni.weak' (Γ := {A}) (by grind)
 
 theorem Derivable.tne {A B : Proposition Atom} :
-    SDerivable ⟨{((A.impl B).impl B).impl B}, A.impl B⟩ := sDerivable_iff.mpr ⟨Derivation.tne⟩
+    SDerivable ⟨{((A ⟶ B) ⟶ B) ⟶ B}, A ⟶ B⟩ := sDerivable_iff.mpr ⟨Derivation.tne⟩
 
 def tneEquiv {A B : Proposition Atom} :
-    Proposition.equiv (A.impl B) (((A.impl B).impl B).impl B) := ⟨Derivation.dni, Derivation.tne⟩
+    Proposition.equiv (A ⟶ B) (((A ⟶ B) ⟶ B) ⟶ B) := ⟨Derivation.dni, Derivation.tne⟩
 
 theorem tne_equivalent {A B : Proposition Atom} :
-    Equiv (A.impl B) (((A.impl B).impl B).impl B) := equiv_iff.mpr ⟨tneEquiv⟩
+    (A ⟶ B) ≡ (((A ⟶ B) ⟶ B) ⟶ B) := equiv_iff.mpr ⟨tneEquiv⟩
 
 /-- Modus tollens -/
 def Derivation.modusTollens {Γ : Ctx Atom} {A B : Proposition Atom} (C : Proposition Atom)
-    (D : Derivation ⟨insert A Γ, B⟩) : Derivation ⟨insert (B.impl C) Γ, A.impl C⟩ :=
+    (D : Derivation ⟨insert A Γ, B⟩) : Derivation ⟨insert (B ⟶ C) Γ, A ⟶ C⟩ :=
   implI _ <|
   implE (A := B)
     (ax' (by grind))
     (D.weak' (h := by grind))
 
 theorem Derivable.modus_tollens {Γ : Ctx Atom} {A B : Proposition Atom} (C : Proposition Atom)
-    (h : SDerivable ⟨insert A Γ, B⟩) : SDerivable ⟨insert (B.impl C) Γ, A.impl C⟩ :=
+    (h : (insert A Γ) ⊢ B) : (insert (B ⟶ C) Γ) ⊢ (A ⟶ C) :=
   let ⟨D⟩ := sDerivable_iff.mp h; sDerivable_iff.mpr ⟨D.modusTollens C⟩
 
 /-!
@@ -82,53 +82,53 @@ The following are valid in minimal logic, so we use `impl (-) C` over `~(-) := i
 
 /-- (A → C) ∧ (B → C) ⊢ (A ∨ B) → C -/
 def disjImpOfConjImps {A B C : Proposition Atom} :
-    Derivation ⟨{conj (impl A C) (impl B C)}, impl (disj A B) C⟩ :=
+    Derivation ⟨{(A ⟶ C) ⋏ (B ⟶ C)}, (A ⋎ B) ⟶ C⟩ :=
   implI _ <|
   disjE (A := A) (B := B)
     (ax _ _)
     (implE (A := A)
-      (conjE₁ (B := B.impl C) (ax' <| by grind))
+      (conjE₁ (B := B ⟶ C) (ax' <| by grind))
       (ax _ _))
     (implE (A := B)
-      (conjE₂ (A := A.impl C) (ax' (by grind)))
+      (conjE₂ (A := A ⟶ C) (ax' (by grind)))
       (ax _ _))
 
 /-- (A → C) ∧ (B → C) ⊢ (A ∨ B) → C -/
 theorem disj_imp_of_conj_imps {A B C : Proposition Atom} :
-    SDerivable ⟨{conj (impl A C) (impl B C)}, impl (disj A B) C⟩ :=
+    {(A ⟶ C) ⋏ (B ⟶ C)} ⊢ ((A ⋎ B) ⟶ C) :=
   sDerivable_iff.mpr ⟨disjImpOfConjImps⟩
 
 /-- (A ∨ B) → C ⊢ (A → C) ∧ (B → C) -/
 def conjImpsOfDisjImp {A B C : Proposition Atom} :
-    Derivation ⟨{impl (disj A B) C}, conj (impl A C) (impl B C)⟩ :=
+    Derivation ⟨{(A ⋎ B) ⟶ C}, (A ⟶ C) ⋏ (B ⟶ C)⟩ :=
   conjI
-    (implI {impl (disj A B) C} <|
-      implE (A := A.disj B) (B := C)
+    (implI {(A ⋎ B) ⟶ C} <|
+      implE (A := A ⋎ B) (B := C)
         (ax' (by grind))
         (disjI₁ (ax _ _)))
-    (implI {impl (disj A B) C} <|
-      implE (A := A.disj B) (B := C)
+    (implI {(A ⋎ B) ⟶ C} <|
+      implE (A := A ⋎ B) (B := C)
         (ax' (by grind))
         (disjI₂ (ax _ _)))
 
 /-- (A ∨ B) → C ⊢ (A → C) ∧ (B → C) -/
 theorem conj_imps_of_disj_imp {A B C : Proposition Atom} :
-    SDerivable ⟨{impl (disj A B) C}, conj (impl A C) (impl B C)⟩ :=
+    SDerivable ⟨{(A ⋎ B) ⟶ C}, (A ⟶ C) ⋏ (B ⟶ C)⟩ :=
   sDerivable_iff.mpr ⟨conjImpsOfDisjImp⟩
 
 def disjImpConjImpsEquiv {A B C : Proposition Atom} :
-    Proposition.equiv (impl (disj A B) C) (conj (impl A C) (impl B C)) :=
+    Proposition.equiv ((A ⋎ B) ⟶ C) ((A ⟶ C) ⋏ (B ⟶ C)) :=
   ⟨conjImpsOfDisjImp, disjImpOfConjImps⟩
 
 theorem disj_imp_conj_imps_equivalent {A B C : Proposition Atom} :
-    Equiv (impl (disj A B) C) (conj (impl A C) (impl B C)) :=
+    Equiv ((A ⋎ B) ⟶ C) ((A ⟶ C) ⋏ (B ⟶ C)) :=
   equiv_iff.mpr ⟨disjImpConjImpsEquiv⟩
 
 /-- (A → C) ∨ (B → C) ⊢ (A ∧ B) → C -/
 def conjImpOfDisjImps {A B C : Proposition Atom} :
-    Derivation ⟨{disj (impl A C) (impl B C)}, impl (conj A B) C⟩ := by
+    Derivation ⟨{(A ⟶ C) ⋎ (B ⟶ C)}, (A ⋏ B) ⟶ C⟩ := by
   apply implI
-  apply disjE (A := A.impl C) (B := B.impl C)
+  apply disjE (A := A ⟶ C) (B := B ⟶ C)
   · exact ax' (by grind)
   · apply implE (A := A)
     · apply ax
@@ -141,13 +141,13 @@ def conjImpOfDisjImps {A B C : Proposition Atom} :
 
 /-- (A → C) ∨ (B → C) ⊢ (A ∧ B) → C -/
 theorem conj_imp_of_disj_imps {A B C : Proposition Atom} :
-    SDerivable ⟨{disj (impl A C) (impl B C)}, impl (conj A B) C⟩ :=
+    SDerivable ⟨{(A ⟶ C) ⋎ (B ⟶ C)}, (A ⋏ B) ⟶ C⟩ :=
   sDerivable_iff.mpr ⟨conjImpOfDisjImps⟩
 
 /-! ### Classical theorems -/
 
 theorem dn_equiv {T : Theory Atom} [IsClassical T] (A : Proposition Atom) :
-    T.Equiv A ((A.impl bot).impl bot) := by
+    T.Equiv A (~~A) := by
   constructor
   · refine ⟨∅, by grind, ?_⟩
     apply implI
@@ -156,78 +156,77 @@ theorem dn_equiv {T : Theory Atom} [IsClassical T] (A : Proposition Atom) :
     grind [IsClassical]
 
 theorem lem {T : Theory Atom} [IsClassical T] {A : Proposition Atom} :
-    T.Derivable (A.disj (A.impl bot)) := by
+    T.Derivable (A ⋎ ~A) := by
   apply Theory.Derivable.dne
   apply Theory.Derivable.theory_weak (T := Theory.empty Atom) (hT := by grind)
   exact Derivable.not_not_lem
 
-private def dneFor (A : Proposition Atom) := ((A.impl bot).impl bot).impl A
+private def dneFor (A : Proposition Atom) := ~~A ⟶ A
 
 theorem disj_not_of_not_conj {T : Theory Atom} [IsClassical T] {A B : Proposition Atom} :
-    T.SDerivable ⟨{(conj A B).impl bot}, disj (A.impl bot) (B.impl bot)⟩ := by
-  refine ⟨{(conj A B).impl bot,
-           dneFor A,
-           dneFor B,
-           dneFor (disj (A.impl bot) (B.impl bot))}, ?_, ?_⟩
+    T.SDerivable ⟨{~(A ⋏ B)}, ~A ⋎ ~B⟩ := by
+  refine ⟨{~(A ⋏ B), dneFor A, dneFor B, dneFor (~A ⋎ ~B)}, ?_, ?_⟩
   · grind [IsClassical, dneFor, Finset.coe_insert, Finset.coe_singleton]
   · simp only [dneFor]
-    apply implE (A := ((disj (A.impl bot) (B.impl bot)).impl bot).impl bot)
+    apply implE (A := ~~(~A ⋎ ~B))
     · exact ax' (by grind)
     · apply implI
-      apply implE (A := A.conj B)
+      apply implE (A := A ⋏ B)
       · exact ax' (by grind)
       · apply conjI
-        · apply implE (A := (A.impl bot).impl bot)
+        · apply implE (A := ~~A)
           · exact ax' (by grind)
           · apply implI
-            apply implE (A := (disj (A.impl bot) (B.impl bot)))
+            apply implE (A := (~A ⋎ ~B))
             · exact ax' (by grind)
             · apply disjI₁
               exact ax' (by grind)
-        · apply implE (A := (B.impl bot).impl bot)
+        · apply implE (A := ~~B)
           · exact ax' (by grind)
           · apply implI
-            apply implE (A := (disj (A.impl bot) (B.impl bot)))
+            apply implE (A := (~A ⋎ ~B))
             · exact ax' (by grind)
             · apply disjI₂
               exact ax' (by grind)
 
 theorem impl_equiv_disj {T : Theory Atom} [IsClassical T] {A B : Proposition Atom} :
-    T.Equiv (A.impl B) ((A.impl bot).disj B) := by
+    (A ⟶ B) ≡[T] (~A ⋎ B) := by
   constructor
   · let ⟨Γ, h, D⟩ := lem (T := T) (A := A)
     refine ⟨Γ, h, ?_⟩
     apply implI
-    apply disjE (A := A) (B := A.impl bot)
+    apply disjE (A := A) (B := ~A)
     · exact D.weak' (by grind)
     · apply disjI₂
       apply implE (A := A)
       all_goals exact ax' (by grind)
     · apply disjI₁
       exact ax ..
-  · refine ⟨{bot.impl B}, by grind [IsClassical], ?_⟩
+  · refine ⟨{⊥ ⟶ B}, by grind [IsClassical], ?_⟩
     apply implI
     apply implI
-    apply disjE (A := A.impl bot) (B := B)
+    apply disjE (A := ~A) (B := B)
     · exact ax' (by grind)
-    · apply implE (A := bot)
+    · apply implE (A := ⊥)
       · exact ax' (by grind)
       · apply implE (A := A)
-        all_goals exact ax' (by grind)
+        all_goals apply ax'
+        · simp [Bot.bot]
+        · grind
     · exact ax' (by grind)
 
 theorem pierce {T : Theory Atom} [IsClassical T] {A B : Proposition Atom} :
-    T.Derivable (((A.impl B).impl A).impl A) := by
+    T.Derivable (((A ⟶ B) ⟶ A) ⟶ A) := by
   let ⟨Γ, h, D⟩ := lem (T := T) (A := A)
-  refine ⟨insert (bot.impl B) Γ, by grind [IsClassical], ?_⟩
+  refine ⟨insert (⊥ ⟶ B) Γ, by grind [IsClassical], ?_⟩
   apply implI
-  apply disjE (A := A) (B := A.impl bot)
+  apply disjE (A := A) (B := A ⟶ ⊥)
   · exact D.weak' (by grind)
   · exact ax ..
-  · apply implE (A := A.impl B)
+  · apply implE (A := A ⟶ B)
     · exact ax' (by grind)
     · apply implI
-      apply implE (A := bot)
+      apply implE (A := ⊥)
       · apply ax' (by grind)
       · apply implE (A := A)
         · exact ax' (by grind)
@@ -238,7 +237,7 @@ theorem pierce {T : Theory Atom} [IsClassical T] {A B : Proposition Atom} :
 
 /-- Equivalence of A → (B → C) and (A ∧ B) → C -/
 def curryEquiv {A B C : Proposition Atom} :
-    Proposition.equiv (A.impl (B.impl C)) (impl (A.conj B) C) := by
+    Proposition.equiv (A ⟶ (B ⟶ C)) ((A ⋏ B) ⟶ C) := by
   constructor
   · apply implI
     apply implE (A := B)
@@ -250,16 +249,16 @@ def curryEquiv {A B C : Proposition Atom} :
       exact ax' (by grind)
   · apply implI
     apply implI
-    apply implE (A := A.conj B)
+    apply implE (A := A ⋏ B)
     · exact ax' (by grind)
     · apply conjI <;> exact ax' (by grind)
 
 /-- Equivalence of A → (B → C) and (A ∧ B) → C -/
 theorem curry_equiv {A B C : Proposition Atom} :
-    Equiv (A.impl (B.impl C)) (impl (A.conj B) C) := equiv_iff.mpr ⟨curryEquiv⟩
+    Equiv (A ⟶ (B ⟶ C)) ((A ⋏ B) ⟶ C) := equiv_iff.mpr ⟨curryEquiv⟩
 
 /-- A ∧ B ⊢ B ∧ A -/
-def conjCommDer {A B : Proposition Atom} : Derivation ⟨{A.conj B}, B.conj A⟩ := by
+def conjCommDer {A B : Proposition Atom} : Derivation ⟨{A ⋏ B}, B ⋏ A⟩ := by
   apply conjI
   · apply conjE₂ (A := A)
     exact ax' (by grind)
@@ -267,26 +266,26 @@ def conjCommDer {A B : Proposition Atom} : Derivation ⟨{A.conj B}, B.conj A⟩
     exact ax' (by grind)
 
 /-- Equivalence of A ∧ B and B ∧ A -/
-def conjCommEquiv {A B : Proposition Atom} : Proposition.equiv (A.conj B) (B.conj A) :=
+def conjCommEquiv {A B : Proposition Atom} : Proposition.equiv (A ⋏ B) (B ⋏ A) :=
   ⟨conjCommDer, conjCommDer⟩
 
 /-- Equivalence of A ∧ B and B ∧ A -/
-theorem conj_comm_equiv {A B : Proposition Atom} : Equiv (A.conj B) (B.conj A) :=
+theorem conj_comm_equiv {A B : Proposition Atom} : (A ⋏ B) ≡ (B ⋏ A) :=
   equiv_iff.mpr ⟨conjCommEquiv⟩
 
 /-- Equivalence of A ∧ A and A -/
-def conjIdemEquiv {A : Proposition Atom} : Proposition.equiv (A.conj A) A := by
+def conjIdemEquiv {A : Proposition Atom} : Proposition.equiv (A ⋏ A) A := by
   constructor
   · apply conjE₁ (B := A)
     exact ax' (by grind)
   · apply conjI <;> exact ax' (by grind)
 
 /-- Equivalence of A ∧ A and A -/
-theorem conj_idem_equiv {A : Proposition Atom} : Equiv (A.conj A) A :=
+theorem conj_idem_equiv {A : Proposition Atom} : (A ⋏ A) ≡ A :=
   equiv_iff.mpr ⟨conjIdemEquiv⟩
 
 /-- A ∨ B ⊢ B ∨ A -/
-def disjCommDer {A B : Proposition Atom} : Derivation ⟨{A.disj B}, B.disj A⟩ := by
+def disjCommDer {A B : Proposition Atom} : Derivation ⟨{A ⋎ B}, B ⋎ A⟩ := by
   apply disjE (A := A) (B := B)
   · exact ax' (by grind)
   · apply disjI₂
@@ -295,27 +294,27 @@ def disjCommDer {A B : Proposition Atom} : Derivation ⟨{A.disj B}, B.disj A⟩
     exact ax' (by grind)
 
 /-- Equivalence of A ∨ B and B ∨ A -/
-def disjCommEquiv {A B : Proposition Atom} : Proposition.equiv (A.disj B) (B.disj A) :=
+def disjCommEquiv {A B : Proposition Atom} : Proposition.equiv (A ⋎ B) (B ⋎ A) :=
   ⟨disjCommDer, disjCommDer⟩
 
 /-- Equivalence of A ∨ B and B ∨ A -/
-theorem disj_comm_equiv {A B : Proposition Atom} : Equiv (A.disj B) (B.disj A) :=
+theorem disj_comm_equiv {A B : Proposition Atom} : (A ⋎ B) ≡ (B ⋎ A) :=
   equiv_iff.mpr ⟨disjCommEquiv⟩
 
 /-- Equivalence of A ∨ A and A -/
-def disjIdemEquiv {A : Proposition Atom} : Proposition.equiv (A.disj A) A := by
+def disjIdemEquiv {A : Proposition Atom} : Proposition.equiv (A ⋎ A) A := by
   constructor
   · apply disjE (A := A) (B := A) <;> exact ax' (by grind)
   · apply disjI₁
     exact ax' (by grind)
 
 /-- Equivalence of A ∨ A and A -/
-theorem disj_idem_equiv {A : Proposition Atom} : Equiv (A.disj A) A :=
+theorem disj_idem_equiv {A : Proposition Atom} : (A ⋎ A) ≡ A :=
   equiv_iff.mpr ⟨disjIdemEquiv⟩
 
 /-- Equivalence of A → (A → B) and A → B -/
 def implIdemEquiv {A B : Proposition Atom} :
-    Proposition.equiv (A.impl <| A.impl B) (A.impl B) := by
+    Proposition.equiv (A ⟶ (A ⟶ B)) (A ⟶ B) := by
   constructor
   · apply implI
     apply implE (A := A)
@@ -328,11 +327,11 @@ def implIdemEquiv {A B : Proposition Atom} :
 
 /-- Equivalence of A → (A → B) and A → B -/
 theorem impl_idem_equiv {A B : Proposition Atom} :
-    Equiv (A.impl <| A.impl B) (A.impl B) := equiv_iff.mpr ⟨implIdemEquiv⟩
+    Equiv (A ⟶ (A ⟶ B)) (A ⟶ B) := equiv_iff.mpr ⟨implIdemEquiv⟩
 
 /-- A → (B → C) ⊢ B → (A → C) -/
 def implSwapDer {A B C : Proposition Atom} :
-    Derivation ⟨{A.impl <| B.impl C}, B.impl (A.impl C)⟩ := by
+    Derivation ⟨{A ⟶ (B ⟶ C)}, B ⟶ (A ⟶ C)⟩ := by
   apply implI
   apply implI
   apply implE (A := B)
@@ -341,27 +340,27 @@ def implSwapDer {A B C : Proposition Atom} :
 
 /-- Equivalence of A → (B → C) and B → (A → C) -/
 def implSwapEquiv {A B C : Proposition Atom} :
-    Proposition.equiv (A.impl <| B.impl C) (B.impl (A.impl C)) := ⟨implSwapDer, implSwapDer⟩
+    Proposition.equiv (A ⟶ (B ⟶ C)) (B ⟶ (A ⟶ C)) := ⟨implSwapDer, implSwapDer⟩
 
 /-- Equivalence of A → (B → C) and B → (A → C) -/
 theorem impl_swap_equiv {A B C : Proposition Atom} :
-    Equiv (A.impl <| B.impl C) (B.impl (A.impl C)) := equiv_iff.mpr ⟨implSwapEquiv⟩
+    (A ⟶ (B ⟶ C)) ≡ (B ⟶ (A ⟶ C)) := equiv_iff.mpr ⟨implSwapEquiv⟩
 
 /-- A → (B → C) ⊢ (A → B) → (A → C) -/
 def implImplDistrib {A B C : Proposition Atom} :
-    Derivation ⟨{A.impl (B.impl C)}, impl (A.impl B) (A.impl C)⟩ := by
+    Derivation ⟨{A ⟶ (B ⟶ C)}, (A ⟶ B) ⟶ (A ⟶ C)⟩ := by
   apply implI
   apply implI
   apply implE (A := B) <;> apply implE (A := A) <;> exact ax' (by grind)
 
 theorem impl_impl_distrib {A B C : Proposition Atom} :
-    SDerivable ⟨{A.impl (B.impl C)}, impl (A.impl B) (A.impl C)⟩ :=
+    {A ⟶ (B ⟶ C)} ⊢ ((A ⟶ B) ⟶ (A ⟶ C)) :=
   sDerivable_iff.mpr ⟨implImplDistrib⟩
 
 /-- Equivalence of A ∧ (A ∨ B) and A -/
-def absorbConjDisj {A B : Proposition Atom} : Proposition.equiv (A.conj <| (A.disj B)) A := by
+def absorbConjDisj {A B : Proposition Atom} : Proposition.equiv (A ⋏ (A ⋎ B)) A := by
   constructor
-  · apply conjE₁ (B := (A.disj B))
+  · apply conjE₁ (B := (A ⋎ B))
     exact ax' (by grind)
   · apply conjI
     · exact ax' (by grind)
@@ -369,13 +368,13 @@ def absorbConjDisj {A B : Proposition Atom} : Proposition.equiv (A.conj <| (A.di
       exact ax' (by grind)
 
 /-- Equivalence of A ∧ (A ∨ B) and A -/
-theorem absorb_conj_disj {A B : Proposition Atom} : Equiv (A.conj <| (A.disj B)) A :=
+theorem absorb_conj_disj {A B : Proposition Atom} : (A ⋏ (A ⋎ B)) ≡ A :=
   equiv_iff.mpr ⟨absorbConjDisj⟩
 
 /-- Equivalence of A ∨ (A ∧ B) and A -/
-def absorbDisjConj {A B : Proposition Atom} : Proposition.equiv (A.disj <| A.conj B) A := by
+def absorbDisjConj {A B : Proposition Atom} : Proposition.equiv (A ⋎ (A ⋏ B)) A := by
   constructor
-  · apply disjE (A := A) (B := A.conj B)
+  · apply disjE (A := A) (B := A ⋏ B)
     · exact ax' (by grind)
     · exact ax' (by grind)
     · apply conjE₁ (B := B)
@@ -384,35 +383,35 @@ def absorbDisjConj {A B : Proposition Atom} : Proposition.equiv (A.disj <| A.con
     exact ax' (by grind)
 
 /-- Equivalence of A ∨ (A ∧ B) and A -/
-theorem absorb_disj_conj {A B : Proposition Atom} :  Equiv (A.disj <| A.conj B) A :=
+theorem absorb_disj_conj {A B : Proposition Atom} :  (A ⋎ (A ⋏ B)) ≡ A :=
   equiv_iff.mpr ⟨absorbDisjConj⟩
 
 /-- Falsum is absorbing for conjunction -/
 theorem bot_conj_absorb (T : Theory Atom) {A : Proposition Atom} [IsIntuitionistic T] :
-  T.Equiv (A.conj bot) bot := by
+  (A ⋏ ⊥) ≡[T] ⊥ := by
   constructor
   · refine ⟨∅, by grind, ?_⟩
     apply implI
     apply conjE₂ (A := A)
     exact ax' (by grind)
-  · refine ⟨{bot.impl A}, by grind [IsIntuitionistic], ?_⟩
+  · refine ⟨{⊥ ⟶ A}, by grind [IsIntuitionistic], ?_⟩
     apply implI
     apply conjI
-    · apply implE (A := bot)
+    · apply implE (A := ⊥)
       · exact ax' (by grind)
       · exact ax ..
     · exact ax' (by grind)
 
 /-- Falsum is neutral for disjunction -/
 theorem bot_disj_neutral (T : Theory Atom) {A : Proposition Atom} [IsIntuitionistic T] :
-    T.Equiv (A.disj bot) A := by
+    (A ⋎ ⊥) ≡[T] A := by
   constructor
-  · refine ⟨{impl bot A}, by grind [IsIntuitionistic], ?_⟩
+  · refine ⟨{⊥ ⟶ A}, by grind [IsIntuitionistic], ?_⟩
     apply implI
-    apply disjE (A := A) (B := bot)
+    apply disjE (A := A) (B := ⊥)
     · exact ax' (by grind)
     · exact ax' (by grind)
-    · apply implE (A := bot)
+    · apply implE (A := ⊥)
       · exact ax' (by grind)
       · exact ax' (by grind)
   · refine ⟨∅, by grind, ?_⟩
@@ -430,25 +429,25 @@ section OrderTheory
 
 variable (T : Theory Atom)
 
-theorem Theory.le_wd {A A' B B' : Proposition Atom} (hA : T.Equiv A A') (hB : T.Equiv B B') :
-    T.Derivable (A.impl B) ↔ T.Derivable (A'.impl B') := by
+theorem Theory.le_wd {A A' B B' : Proposition Atom} (hA : A ≡[T] A') (hB : B ≡[T] B') :
+    ⊢[T] (A ⟶ B) ↔ ⊢[T] (A'.impl B') := by
   constructor <;> intro h
   · exact hA.2.trans h |>.trans hB.1
   · exact hA.1.trans h |>.trans hB.2
 
-theorem Theory.le_refl {A : Proposition Atom} : T.Derivable (A.impl A) := by
+theorem Theory.le_refl {A : Proposition Atom} : ⊢[T] (A ⟶ A) := by
   refine ⟨∅, by grind, ?_⟩
   apply implI
   exact ax _ _
 
-theorem Theory.le_trans {A B C : Proposition Atom} (hAB : T.Derivable (A.impl B))
-    (hBC : T.Derivable (B.impl C)) : T.Derivable (A.impl C) := hAB.trans hBC
+theorem Theory.le_trans {A B C : Proposition Atom} (hAB : ⊢[T] (A ⟶ B))
+    (hBC : ⊢[T] (B ⟶ C)) : ⊢[T] (A ⟶ C) := hAB.trans hBC
 
-theorem Theory.le_antisymm {A B : Proposition Atom} (hAB : T.Derivable (A.impl B))
-    (hBA : T.Derivable (B.impl A)) : T.Equiv A B := ⟨hAB, hBA⟩
+theorem Theory.le_antisymm {A B : Proposition Atom} (hAB : ⊢[T] (A ⟶ B))
+    (hBA : ⊢[T] (B ⟶ A)) : A ≡[T] B := ⟨hAB, hBA⟩
 
 theorem Theory.inf_wd {A A' B B' : Proposition Atom} :
-    T.Equiv A A' → T.Equiv B B' → T.Equiv (A.conj B) (A'.conj B')
+    A ≡[T] A' → B ≡[T] B' → (A ⋏ B) ≡[T] (A' ⋏ B')
   | ⟨⟨ΓA, hA, DA⟩, ⟨ΓA', hA', DA'⟩⟩, ⟨⟨ΓB, hB, DB⟩, ⟨ΓB', hB', DB'⟩⟩ => by
     constructor
     · refine ⟨ΓA ∪ ΓB, by grind, ?_⟩
@@ -475,7 +474,7 @@ theorem Theory.inf_wd {A A' B B' : Proposition Atom} :
           apply ax' (by grind)
 
 theorem Theory.sup_wd {A A' B B' : Proposition Atom} :
-    T.Equiv A A' → T.Equiv B B' → T.Equiv (A.disj B) (A'.disj B')
+    A ≡[T] A' → B ≡[T] B' → (A ⋎ B) ≡[T] (A' ⋎ B')
   | ⟨⟨ΓA, hA, DA⟩, ⟨ΓA', hA', DA'⟩⟩, ⟨⟨ΓB, hB, DB⟩, ⟨ΓB', hB', DB'⟩⟩ => by
     constructor
     · refine ⟨ΓA ∪ ΓB, by grind, ?_⟩
@@ -501,20 +500,20 @@ theorem Theory.sup_wd {A A' B B' : Proposition Atom} :
         · exact DB'.weak' (by grind)
         · exact ax ..
 
-theorem Theory.inf_le_left {A B : Proposition Atom} : T.Derivable ((A.conj B).impl A) := by
+theorem Theory.inf_le_left {A B : Proposition Atom} : ⊢[T] ((A ⋏ B) ⟶ A) := by
   refine ⟨∅, by grind, ?_⟩
   apply implI
   apply conjE₁ (B := B)
   exact ax ..
 
-theorem Theory.inf_le_right {A B : Proposition Atom} : T.Derivable ((A.conj B).impl B) := by
+theorem Theory.inf_le_right {A B : Proposition Atom} : ⊢[T] ((A ⋏ B) ⟶ B) := by
   refine ⟨∅, by grind, ?_⟩
   apply implI
   apply conjE₂ (A := A)
   exact ax ..
 
 theorem Theory.le_inf {A B C : Proposition Atom} :
-    T.Derivable (A.impl B) → T.Derivable (A.impl C) → T.Derivable (A.impl (B.conj C))
+    ⊢[T] (A ⟶ B) → ⊢[T] (A ⟶ C) → ⊢[T] (A ⟶ (B ⋏ C))
   | ⟨Γ, h, D⟩, ⟨Γ', h', D'⟩ => by
     refine ⟨Γ ∪ Γ', by grind, ?_⟩
     apply implI
@@ -526,20 +525,20 @@ theorem Theory.le_inf {A B C : Proposition Atom} :
       · exact D'.weak' (by grind)
       · exact ax ..
 
-theorem Theory.le_sup_left {A B : Proposition Atom} : T.Derivable (A.impl (A.disj B)) := by
+theorem Theory.le_sup_left {A B : Proposition Atom} : ⊢[T] (A ⟶ (A ⋎ B)) := by
   refine ⟨∅, by grind, ?_⟩
   apply implI
   apply disjI₁
   exact ax ..
 
-theorem Theory.le_sup_right {A B : Proposition Atom} : T.Derivable (B.impl (A.disj B)) := by
+theorem Theory.le_sup_right {A B : Proposition Atom} : ⊢[T] (B ⟶ (A ⋎ B)) := by
   refine ⟨∅, by grind, ?_⟩
   apply implI
   apply disjI₂
   exact ax ..
 
 theorem Theory.sup_le {A B C : Proposition Atom} :
-    T.Derivable (A.impl C) → T.Derivable (B.impl C) → T.Derivable (A.disj B |>.impl C)
+    ⊢[T] (A ⟶ C) → ⊢[T] (B ⟶ C) → ⊢[T] (A ⋎ B ⟶ C)
   | ⟨Γ, h, D⟩, ⟨Γ', h', D'⟩ => by
     refine ⟨Γ ∪ Γ', by grind, ?_⟩
     apply implI
@@ -552,16 +551,16 @@ theorem Theory.sup_le {A B C : Proposition Atom} :
       · exact D'.weak' (by grind)
       · exact ax ..
 
-theorem Theory.le_top {A : Proposition Atom} : T.Derivable (A.impl Proposition.top) := by
+theorem Theory.le_top {A : Proposition Atom} : T.Derivable (A ⟶ ⊤) := by
   refine ⟨∅, by grind, ?_⟩
   apply implI
   exact derivationTop.weak' (by grind)
 
-theorem Theory.bot_le {A : Proposition Atom} [IsIntuitionistic T] : T.Derivable (bot.impl A) :=
+theorem Theory.bot_le {A : Proposition Atom} [IsIntuitionistic T] : T.Derivable (⊥ ⟶ A) :=
   Theory.Derivable.ax' (by grind [IsIntuitionistic])
 
 theorem Theory.himp_wd {A A' B B' : Proposition Atom} :
-    T.Equiv A A' → T.Equiv B B' → T.Equiv (A.impl B) (A'.impl B')
+    A ≡[T] A' → B ≡[T] B' → (A ⟶ B) ≡[T] (A' ⟶ B')
   | ⟨⟨ΓA, hA, DA⟩, ⟨ΓA', hA', DA'⟩⟩, ⟨⟨ΓB, hB, DB⟩, ⟨ΓB', hB', DB'⟩⟩ => by
     constructor
     · refine ⟨ΓA' ∪ ΓB, by grind, ?_⟩
@@ -584,7 +583,7 @@ theorem Theory.himp_wd {A A' B B' : Proposition Atom} :
           · exact ax ..
 
 theorem Theory.le_himp_iff {A B C : Proposition Atom} :
-    T.Derivable (A.impl (B.impl C)) ↔ T.Derivable ((A.conj B).impl C) := by
+    ⊢[T] (A ⟶ (B ⟶ C)) ↔ ⊢[T] (A ⋏ B ⟶ C) := by
   apply T.equivalent_derivable
   apply Theory.Equiv.theory_weak (Theory.empty Atom) T (by grind)
   exact curry_equiv
